prim/prim.c
@@ -36,7 +36,7 @@ IMPORTANT: The soundness of the graph depends on declaring evalid g (u,v) -> u <
     otherwise algorithm doesn't preserve whether (u,v) or (v,u) is in graph
 It's not even clear in a conventional adjacency matrix anyway, because an undirected adjmatrix is symmetrical ("nice" graphs)
 */
-int prim(int graph[SIZE][SIZE], int parent[SIZE]) {
+void prim(int graph[SIZE][SIZE], int r, int parent[SIZE]) {
     //This should ideally be replaced by a pq-specific "find_item_in_queue", but depending on the pq may be O(logn)
     int key[SIZE];
     initialise_list(key, IFTY);
@@ -44,6 +44,7 @@ int prim(int graph[SIZE][SIZE], int parent[SIZE]) {
     //as a marker to check if v is in pq. 1 for NOT in pq (already checked). This should ideally be replaced by a pq-specific "in_queue"
     int out[SIZE];
     initialise_list(out, 0);
+    key[r] = 0; //first in pq
     
     //Q = G.V;
     int pq[SIZE];
@@ -55,7 +56,7 @@ int prim(int graph[SIZE][SIZE], int parent[SIZE]) {
         out[u] = 1;
         for (int v = 0; v < SIZE; ++v) {
             if (out[v]==0) {				//(*this is why out array is kept, to not require extra O(logn) search of pq*)
-		if (graph[u][v] < key[v]) { //(*this is why key array is kept, to not require extra O(logn) search of pq*)
+		        if (graph[u][v] < key[v]) { //(*this is why key array is kept, to not require extra O(logn) search of pq*)
 	                parent[v] = u;
 	                key[v] = graph[u][v];
 	                adjustWeight(v, key[v], pq);
@@ -63,5 +64,5 @@ int prim(int graph[SIZE][SIZE], int parent[SIZE]) {
             }
         }
     }
-    return 0;
+    return;
 }
