prim/verif_prim.v
@@ -3,13 +3,14 @@ Require Import CertiGraph.lib.List_ext.
 Require Import CertiGraph.floyd_ext.share.
 Require Import CertiGraph.graph.graph_model.
 Require Import CertiGraph.graph.graph_relation.
-Require Import CertiGraph.graph.undirected_graph.
-Require Import CertiGraph.prim.MatrixUGraph.
-Require Import CertiGraph.priq.priq_arr_specs.
-Require Import CertiGraph.priq.priq_arr_utils.
-Require Import CertiGraph.prim.spatial_undirected_matrix.
-Require Import CertiGraph.prim.noroot_prim.
-Require Import CertiGraph.prim.specs_noroot_prim.
+(* Require Import CertiGraph.graph.FiniteGraph. *)
+
+Require Import CertiGraph.graph.undirected_graph. (* uforest' *)
+Require Import CertiGraph.priq.priq_arr_utils. (* find *)
+Require Import CertiGraph.prim.MatrixUGraph. (* vert_bound *)
+Require Import CertiGraph.prim.prim.
+Require Import CertiGraph.prim.spatial_undirected_matrix. (* list_address *)
+Require Import CertiGraph.prim.specs_prim.
 
 Local Open Scope Z.
 
@@ -142,11 +143,8 @@ Qed.
 
 Lemma body_prim: semax_body Vprog Gprog f_prim prim_spec.
 Proof.
-start_function.
+start_function. rename H into Hprecon_1.
 pose proof inf_repable as inf_repable.
-assert (size_repable: repable_signed SIZE). unfold repable_signed. unfold SIZE.
-set (i:=Int.min_signed); compute in i; subst i.
-set (i:=Int.max_signed); compute in i; subst i. lia.
 (*replace all data_at_ with data_at Vundef*)
 repeat rewrite data_at__tarray.
 set (k:=default_val tint); compute in k; subst k.
@@ -155,17 +153,23 @@ assert_PROP (Zlength (map (fun x : Z => Vint (Int.repr x)) garbage) = SIZE). ent
 forward_call (sh, (pointer_val_val parent_ptr), (map (fun x : Z => Vint (Int.repr x)) garbage), SIZE).
 clear H garbage.
 forward_call (Tsh, v_out, (list_repeat (Z.to_nat 8) Vundef), 0).
-assert (Hstarting_keys: forall i, 0 <= i < SIZE -> is_int I32 Signed (Znth i (list_repeat (Z.to_nat SIZE) (Vint (Int.repr inf))))). {
-  intros. unfold is_int. rewrite Znth_list_repeat_inrange by lia. auto.
+assert (Hrbound: 0 <= r < SIZE). apply vert_bound in Hprecon_1; auto.
+forward.
+assert (Hstarting_keys: forall i, 0 <= i < SIZE -> is_int I32 Signed (Znth i (upd_Znth r (list_repeat (Z.to_nat SIZE) (Vint (Int.repr inf))) (Vint (Int.repr 0))))). {
+  intros. unfold is_int. destruct (Z.eq_dec i r).
+  +subst i. rewrite upd_Znth_same. auto. rewrite Zlength_list_repeat; lia.
+  +rewrite Znth_upd_Znth_diff; auto. rewrite Znth_list_repeat_inrange by lia. auto.
 }
-replace (list_repeat (Z.to_nat SIZE) (Vint (Int.repr inf))) with
-  (map (fun x => Vint (Int.repr x)) (list_repeat (Z.to_nat SIZE) inf)) in *.
-set (starting_keys:=map (fun x => Vint (Int.repr x)) (list_repeat (Z.to_nat SIZE) inf)) in *.
+replace (upd_Znth r (list_repeat (Z.to_nat SIZE) (Vint (Int.repr inf))) (Vint (Int.repr 0))) with
+  (map (fun x => Vint (Int.repr x)) (upd_Znth r (list_repeat (Z.to_nat SIZE) inf) 0)) in *.
+2: rewrite (upd_Znth_map (fun x => Vint (Int.repr x)) r (list_repeat (Z.to_nat SIZE) inf)); auto.
+set (starting_keys:=map (fun x => Vint (Int.repr x)) (upd_Znth r (list_repeat (Z.to_nat SIZE) inf) 0)) in *.
 assert (HZlength_starting_keys: Zlength starting_keys = SIZE). {
-  unfold starting_keys. rewrite Zlength_map. rewrite Zlength_list_repeat. lia. pose proof SIZE_rep; lia.
+  unfold starting_keys. rewrite Zlength_map. rewrite Zlength_upd_Znth. rewrite Zlength_list_repeat; lia.
 }
 pose proof SIZE_rep as SIZE_rep.
 unfold repable_signed in inf_repable.
+assert (infpos: 0 < inf). { unfold inf. set (j:=Int.max_signed) in *; compute in j; subst j. lia. }
 (*push all vertices into priq*)
 forward_for_simple_bound SIZE
   (EX i : Z,
@@ -173,7 +177,7 @@ forward_for_simple_bound SIZE
     LOCAL (
       lvar _pq (tarray tint 8) v_pq; lvar _out (tarray tint 8) v_out;
       lvar _key (tarray tint 8) v_key; temp _graph (pointer_val_val gptr);
-      temp _parent (pointer_val_val parent_ptr)
+      temp _r (Vint (Int.repr r)); temp _parent (pointer_val_val parent_ptr)
     )
     SEP (
       data_at Tsh (tarray tint SIZE) (list_repeat (Z.to_nat SIZE) (Vint (Int.repr 0))) v_out;
@@ -186,12 +190,16 @@ forward_for_simple_bound SIZE
 entailer!. (*precon taken care of*)
 (*loop*)
 forward.
-assert (Znth i starting_keys = Vint (Int.repr (Znth i (list_repeat (Z.to_nat SIZE) inf)))). {
+assert (Znth i starting_keys = Vint (Int.repr (Znth i (upd_Znth r (list_repeat (Z.to_nat SIZE) inf) 0)))). {
   unfold starting_keys. rewrite Znth_map; auto.
+  rewrite Zlength_upd_Znth. rewrite Zlength_list_repeat; lia.
 }
-forward_call (v_pq, i, Znth i (list_repeat (Z.to_nat SIZE) inf), sublist 0 i starting_keys ++ sublist i SIZE (list_repeat (Z.to_nat 8) Vundef)).
+forward_call (v_pq, i, Znth i (upd_Znth r (list_repeat (Z.to_nat SIZE) inf) 0), sublist 0 i starting_keys ++ sublist i SIZE (list_repeat (Z.to_nat 8) Vundef)).
 split. auto. unfold weight_inrange_priq.
-rewrite Znth_list_repeat_inrange. lia. lia.
+destruct (Z.eq_dec i r). subst i. rewrite upd_Znth_same. split. pose proof Int.min_signed_neg; lia.
+rewrite inf_eq; lia. rewrite Zlength_list_repeat; lia.
+rewrite upd_Znth_diff, Znth_list_repeat_inrange. lia.
+lia. rewrite Zlength_list_repeat; lia. rewrite Zlength_list_repeat; lia. auto.
 entailer!.
 rewrite upd_Znth_app2. rewrite Zlength_sublist, Z.sub_0_r, Z.sub_diag; try lia.
 rewrite (sublist_split i (i+1) SIZE). rewrite (sublist_one i (i+1)). rewrite upd_Znth_app1.
@@ -207,7 +215,6 @@ rewrite sublist_nil, app_nil_r, sublist_same; try lia.
 rewrite <- (map_list_repeat (fun x => Vint (Int.repr x))).
 rewrite <- (map_list_repeat (fun x => Vint (Int.repr x))).
 pose proof (finGraph g) as fg.
-(*whew! all setup done!*)
 (*now for the pq loop*)
 forward_loop (
   EX mst':G,
@@ -224,7 +231,7 @@ forward_loop (
       (*about the lists*)
       Permutation (popped_vertices++unpopped_vertices) (VList g);
       forall v, 0 <= v < SIZE -> 0 <= Znth v parents <= SIZE;
-      forall v, 0 <= v < SIZE -> Znth v keys = elabel g (eformat (v, Znth v parents));
+      forall v, 0 <= v < SIZE -> Znth v keys = if V_EqDec v r then 0 else elabel g (eformat (v, Znth v parents));
       forall v, 0 <= v < SIZE -> Znth v pq_state = if in_dec V_EqDec v popped_vertices then Z.add inf 1 else Znth v keys;
       forall v, 0 <= v < SIZE -> 0 <= Znth v parents < SIZE ->
           (evalid g (eformat (v, Znth v parents)) /\ (*together you form a valid edge in g*)
@@ -246,12 +253,15 @@ forward_loop (
         ~ In u2 (sublist 0 ((@find V V_EqDec) popped_vertices v 0) popped_vertices) ->
         elabel g (eformat (v, Znth v parents)) <= elabel g (eformat (u1,u2));
       (*minimality...*)
-      exists M, minimum_spanning_forest M g /\ is_partial_lgraph mst' M
+      exists M, minimum_spanning_forest M g /\ is_partial_lgraph mst' M;
+      (*the following two are yuck...*)
+      popped_vertices = nil -> r = (@find Z priq_arr_specs.Z_EqDec) pq_state (fold_right Z.min (hd 0 pq_state) pq_state) 0;
+      popped_vertices <> nil -> hd_error popped_vertices = Some r
     )
     LOCAL (
       lvar _pq (tarray tint 8) v_pq; lvar _out (tarray tint 8) v_out;
       temp _parent (pointer_val_val parent_ptr); lvar _key (tarray tint 8) v_key;
-      temp _graph (pointer_val_val gptr)
+      temp _graph (pointer_val_val gptr); temp _r (Vint (Int.repr r))
     )
     SEP (
       data_at Tsh (tarray tint SIZE) (map (fun x => if in_dec V_EqDec x popped_vertices
@@ -283,6 +293,7 @@ break: (
       (*something about weight*)
       Permutation (EList mst) (map (fun v => eformat (v, Znth v parents)) (filter (fun v => Znth v parents <? SIZE) popped_vertices));
       spanning mst g;
+      hd_error popped_vertices = Some r; (*<-idk if necessary, just putting it in in case*)
       (*weight*)
       forall v u1 u2, In v popped_vertices -> 0 <= Znth v parents < SIZE ->
         vvalid g u2 ->
@@ -296,7 +307,7 @@ break: (
     LOCAL (
       lvar _pq (tarray tint 8) v_pq; lvar _out (tarray tint 8) v_out;
       temp _parent (pointer_val_val parent_ptr); lvar _key (tarray tint 8) v_key;
-      temp _graph (pointer_val_val gptr)
+      temp _graph (pointer_val_val gptr); temp _r (Vint (Int.repr r))
     )
     SEP (
       data_at Tsh (tarray tint SIZE) (list_repeat (Z.to_nat SIZE) (Vint (Int.repr 1))) v_out;
@@ -311,8 +322,8 @@ break: (
   Exists edgeless_graph'.
   pose proof (finGraph edgeless_graph') as fe. Exists fe.
   Exists (list_repeat (Z.to_nat SIZE) SIZE).
-  Exists (list_repeat (Z.to_nat SIZE) inf).
-  Exists (list_repeat (Z.to_nat SIZE) inf).
+  Exists (upd_Znth r (list_repeat (Z.to_nat SIZE) inf) 0).
+  Exists (upd_Znth r (list_repeat (Z.to_nat SIZE) inf) 0).
   Exists (nil (A:=V)).
   Exists (VList g). rewrite app_nil_l.
   assert (Hinv_1: is_partial_lgraph edgeless_graph' g). apply edgeless_partial_lgraph.
@@ -321,19 +332,22 @@ break: (
   assert (Hinv_4: forall v : Z, 0 <= v < SIZE -> 0 <= Znth v (list_repeat (Z.to_nat SIZE) SIZE) <= SIZE). {
     intros. rewrite Znth_list_repeat_inrange; lia.
   }
-  assert (Hinv_5: forall v : Z, 0 <= v < SIZE -> Znth v (list_repeat (Z.to_nat SIZE) inf) =
-    elabel g (eformat (v, Znth v (list_repeat (Z.to_nat SIZE) SIZE)))). {
-    intros.
-    repeat rewrite Znth_list_repeat_inrange by lia. symmetry; apply invalid_edge_weight.
+  assert (Hinv_5: forall v : Z, 0 <= v < SIZE -> Znth v (upd_Znth r (list_repeat (Z.to_nat SIZE) inf) 0) =
+    (if V_EqDec v r then 0 else elabel g (eformat (v, Znth v (list_repeat (Z.to_nat SIZE) SIZE))))). {
+    intros. destruct (V_EqDec v r).
+    hnf in e; subst v. rewrite upd_Znth_same. auto. rewrite Zlength_list_repeat; lia.
+    unfold RelationClasses.complement, Equivalence.equiv in c. rewrite upd_Znth_diff.
+    repeat rewrite Znth_list_repeat_inrange by lia. symmetry; rewrite <- (invalid_edge_weight g); auto.
     unfold not; intros. rewrite <- eformat_adj in H0. apply adjacent_requires_vvalid in H0. destruct H0.
     rewrite vert_bound in H1. lia.
+    rewrite Zlength_list_repeat; lia. rewrite Zlength_list_repeat; lia. auto.
   }
   assert (Hinv_6: forall v : Z,
     0 <= v < SIZE ->
-    Znth v (list_repeat (Z.to_nat SIZE) inf) =
+    Znth v (upd_Znth r (list_repeat (Z.to_nat SIZE) inf) 0) =
     (if in_dec V_EqDec v (nil (A:=V))
      then (inf + 1)%Z
-     else Znth v (list_repeat (Z.to_nat SIZE) inf))). {
+     else Znth v (upd_Znth r (list_repeat (Z.to_nat SIZE) inf) 0))). {
     intros. destruct (in_dec V_EqDec v []); [contradiction | auto].
   }
   assert (Hinv_7: forall v : Z, 0 <= v < SIZE ->
@@ -355,14 +369,23 @@ break: (
          (filter (fun v : Z => Znth v (list_repeat (Z.to_nat SIZE) SIZE) <? SIZE) []))). {
     simpl.
     (*because I've trouble using edgeless_graph_EList*) apply NoDup_Permutation. apply NoDup_EList. apply NoDup_nil.
-    intros. rewrite EList_evalid. split; intros. pose proof (@edgeless_graph_evalid inf SIZE inf_rep SIZE_rep' x); contradiction. contradiction.
+    intros. rewrite EList_evalid. split; intros. pose proof (@edgeless_graph_evalid SIZE inf inf_rep SIZE_rep' x); contradiction. contradiction.
+  }
+  assert (Hr1: forall u v : V, In u (nil (A:=V)) -> In v (nil (A:=V)) -> connected g u v <-> connected edgeless_graph' u v). {
+    intros. contradiction.
+  }
+  assert (Hr2: (nil (A:=V)) = (nil (A:=V)) ->
+    r = (@find Z priq_arr_specs.Z_EqDec) (upd_Znth r (list_repeat (Z.to_nat SIZE) inf) 0)
+      (fold_right Z.min (hd 0 (upd_Znth r (list_repeat (Z.to_nat SIZE) inf) 0))
+         (upd_Znth r (list_repeat (Z.to_nat SIZE) inf) 0)) 0). {
+    intros. rewrite find_src. auto. auto. lia.
   }
   (*Hinv_12 (nil <> nil) seems to be missing, autoresolved?*)
-  assert (Hinv_11: forall u v : V, In u (VList g) -> ~ adjacent edgeless_graph' u v). {
+  assert (Hinv_13: forall u v : V, In u (VList g) -> ~ adjacent edgeless_graph' u v). {
     unfold not; intros. destruct H0 as [e [? ?]]. destruct H0.
-    pose proof (@edgeless_graph_evalid inf SIZE inf_rep SIZE_rep' e); contradiction.
+    pose proof (@edgeless_graph_evalid SIZE inf inf_rep SIZE_rep' e); contradiction.
   }
-  assert (Hinv_12: forall v u1 u2 : V,
+  assert (Hinv_14: forall v u1 u2 : V,
     In v (nil (A:=V)) ->
     0 <= Znth v (list_repeat (Z.to_nat SIZE) SIZE) < SIZE ->
     vvalid g u2 ->
@@ -372,7 +395,7 @@ break: (
     elabel g (eformat (u1, u2))). {
     intros. contradiction.
   }
-  assert (Hinv_13: exists M, minimum_spanning_forest M g /\ is_partial_lgraph edgeless_graph' M). {
+  assert (Hinv_15: exists M, minimum_spanning_forest M g /\ is_partial_lgraph edgeless_graph' M). {
     destruct (exists_msf g) as [M ?]. exists M; split. auto.
     apply edgeless_partial_lgraph.
   }
@@ -389,7 +412,8 @@ break: (
     destruct (in_dec V_EqDec i []); [contradiction | auto].
   }
   unfold starting_keys.
-  time "main loop precon:" entailer!.
+  time "main loop precon (originally 446.87s):" entailer!.
+  (*without Hinv_10 and Hinv_12, took 120-200 seconds. I guess entailer doesn't try contradiction early?*)
 }
 (****MAIN LOOP****) {
   clear Hstarting_keys HZlength_starting_keys starting_keys.
@@ -400,8 +424,9 @@ break: (
   rename H3 into Hinv_5; rename H4 into Hinv_6;
   rename H5 into Hinv_7; rename H6 into Hinv_8;
   rename H7 into Hinv_9; rename H8 into Hinv_10;
-  rename H9 into Hinv_11; rename H10 into Hinv_12;
-  rename H11 into Hinv_13.
+  rename H9 into Hinv_13; rename H10 into Hinv_14;
+  rename H11 into Hinv_15; rename H12 into Hr1;
+  rename H13 into Hr2.
   (*15 invariants... I think, that if we go with this "exists M" approach, we can eliminate some of the weight lemmas*)
   assert_PROP (Zlength (map (fun x : Z => Vint (Int.repr x)) parents) = SIZE /\
               Zlength (map (fun x : Z => Vint (Int.repr x)) keys) = SIZE /\
@@ -420,21 +445,21 @@ break: (
     intros. rewrite <- VList_vvalid. apply (Permutation_in (l:=popped_vertices++unpopped_vertices)).
     apply Hinv_3. apply in_or_app; right; auto.
   }
-  assert ((@inrange_priq inf) pq_state). {
-    unfold inrange_priq. rewrite Forall_forall. intros x Hx.
+  assert ((@priq_arr_utils.inrange_priq inf) pq_state). {
+    unfold priq_arr_utils.inrange_priq. rewrite Forall_forall. intros x Hx.
     rewrite In_Znth_iff in Hx. destruct Hx as [i [? ?]]. rewrite HZlength_pq_state in H. subst x.
     rewrite Hinv_6. 2: lia. destruct (in_dec V_EqDec i popped_vertices). lia.
-    rewrite Hinv_5. 2: lia.
+    rewrite Hinv_5. 2: lia. destruct (V_EqDec i r). auto.
     split. apply weight_representable. apply (Z.le_trans _ inf). apply weight_inf_bound. lia.
   }
   replace (data_at Tsh (tarray tint SIZE) (map (fun x : Z => Vint (Int.repr x)) pq_state) v_pq)
     with (data_at Tsh (tarray tint SIZE) (map Vint (map Int.repr pq_state)) v_pq).
-  2: { unfold SIZE, SIZE. rewrite list_map_compose. auto. }
+  2: { unfold SIZE. rewrite list_map_compose. auto. }
   forward_call (v_pq, pq_state).
   forward_if.
   (*PROCEED WITH LOOP*) {
-  assert ((@isEmpty inf) pq_state = Vzero). {
-    destruct ((@isEmptyTwoCases inf) pq_state);
+  assert ((@priq_arr_utils.isEmpty inf) pq_state = Vzero). {
+    destruct ((@priq_arr_utils.isEmptyTwoCases inf) pq_state);
     rewrite H1 in H0; simpl in H0; now inversion H0.
   }
   forward_call (v_pq, pq_state). Intros u. rename H2 into Hu.
@@ -443,7 +468,7 @@ break: (
   assert (0 <= u < SIZE). {
     rewrite Hu. rewrite <- HZlength_pq_state. apply find_range.
     apply min_in_list. apply incl_refl. destruct pq_state.
-    rewrite Zlength_nil in HZlength_pq_state. unfold SIZE in HZlength_pq_state; lia.
+    rewrite Zlength_nil in HZlength_pq_state. lia.
     simpl. left; trivial.
   }
   assert (Hu_not_popped: ~ In u popped_vertices). { unfold not; intros.
@@ -452,7 +477,7 @@ break: (
     destruct (in_dec V_EqDec u popped_vertices). lia. contradiction.
   }
   assert (Hu_unpopped: In u unpopped_vertices). { destruct (Hpopped_or_unpopped u).
-    rewrite vvalid_meaning. auto. contradiction. auto.
+    rewrite (vvalid_meaning g). auto. contradiction. auto.
   }
   forward.
   replace (upd_Znth u (map (fun x : V =>
@@ -481,6 +506,9 @@ break: (
   }
   rewrite upd_Znth_map. rewrite upd_Znth_map. rewrite list_map_compose. (*pq state*)
   replace (Znth 0 pq_state) with (hd 0 pq_state). rewrite <- Hu. 2: { destruct pq_state. rewrite Zlength_nil in HZlength_pq_state; lia. simpl. rewrite Znth_0_cons. auto. }
+  assert (Hur: popped_vertices = nil -> u = r). {
+    intros. rewrite Hu. symmetry. apply Hr1. auto.
+  }
   assert (Hu_min: forall v, 0 <= v < SIZE -> Znth u pq_state <= Znth v pq_state). {
     intros. rewrite Hu. rewrite Znth_find.
     apply fold_min. apply Znth_In. lia.
@@ -516,7 +544,8 @@ break: (
       )
       LOCAL (
         temp _u (Vint (Int.repr u)); temp _t'1 ((@isEmpty inf) pq_state); lvar _pq (tarray tint 8) v_pq; lvar _out (tarray tint 8) v_out;
-        temp _parent (pointer_val_val parent_ptr); lvar _key (tarray tint 8) v_key; temp _graph (pointer_val_val gptr)
+        temp _parent (pointer_val_val parent_ptr); lvar _key (tarray tint 8) v_key; temp _graph (pointer_val_val gptr);
+        temp _r (Vint (Int.repr r))
       )
       SEP (data_at Tsh (tarray tint SIZE) (map (fun x => Vint (Int.repr x)) pq_state') v_pq;
      data_at Tsh (tarray tint 8)
@@ -533,7 +562,7 @@ break: (
   (*precon*) {
     Exists parents. Exists keys. Exists upd_pq_state. entailer!.
     (*in this case, proving the PROPs beforehand did not improve the timing*)
-    intros. rewrite Hinv_5 by lia. split.
+    intros. rewrite Hinv_5 by lia. destruct (V_EqDec v r). auto. split.
     apply weight_representable. apply weight_inf_bound.
   }
   (*loop*)
@@ -597,7 +626,7 @@ break: (
     entailer!. rewrite list_map_compose. auto.
     split. lia.
     unfold weight_inrange_priq. rewrite graph_to_mat_eq. split.
-    apply weight_representable. rewrite eformat_adj_elabel, eformat_symm in Hadj_ui. lia. lia. lia.
+    apply weight_representable. rewrite eformat_adj_elabel, eformat_symm in Hadj_ui. apply Z.le_lteq. left; apply Hadj_ui. lia. lia.
     Exists (upd_Znth i parents' u).
     Exists (upd_Znth i keys' (Znth i (Znth u (graph_to_symm_mat g)))).
     Exists (upd_Znth i pq_state' (Znth i (Znth u (graph_to_symm_mat g)))).
@@ -771,7 +800,7 @@ break: (
     destruct (Znth u (Znth v (graph_to_symm_mat g)) <? Znth v upd_pq_state) eqn:bool. lia. apply Hinv_4; auto.
     replace (Znth v parents') with (Znth v parents). 2: symmetry; apply Hinv2_1; auto. apply Hinv_4; auto.
   }
-  assert (Hkeys': forall v : Z, 0 <= v < SIZE -> Znth v keys' = elabel g (eformat (v, Znth v parents'))). {
+  assert (Hkeys': forall v : Z, 0 <= v < SIZE -> Znth v keys' = (if V_EqDec v r then 0 else elabel g (eformat (v, Znth v parents')))). {
     intros. destruct (adjacent_dec g u v). destruct (in_dec Z.eq_dec v (popped_vertices +::u)).
     ****
     replace (Znth v keys') with (Znth v keys). 2: symmetry; apply Hinv2_1; auto. rewrite Hinv_5.
@@ -779,12 +808,17 @@ break: (
     ****
     replace (Znth v keys') with (Z.min (elabel g (eformat (u, v))) (Znth v upd_pq_state)). 2: symmetry; apply Hinv2_2; auto.
     replace (Znth v parents') with (if elabel g (eformat (u, v)) <? Znth v upd_pq_state then u else Znth v parents). 2: symmetry; apply Hinv2_2; auto.
+    destruct (V_EqDec v r). hnf in e.
+    (*v=r*) subst v. destruct popped_vertices. exfalso. apply n. apply in_or_app; right; left. apply Hur; auto.
+    assert (hd_error (v :: popped_vertices) = Some r). apply Hr2. unfold not; intros. inversion H7. inversion H7. subst v.
+    exfalso. apply n. apply in_or_app; left; left; auto.
+    (*v <> r*)
     rewrite <- graph_to_mat_eq by lia. destruct (Znth u (Znth v (graph_to_symm_mat g)) <? Znth v upd_pq_state) eqn:bool.
     rewrite graph_to_mat_eq by lia. rewrite graph_to_mat_eq in bool by lia. rewrite Z.ltb_lt in bool. rewrite Zlt_Zmin by auto. rewrite eformat_symm; auto.
     rewrite graph_to_mat_eq by lia. rewrite graph_to_mat_eq in bool by lia. rewrite Z.ltb_ge in bool. rewrite Z.min_r by auto.
     unfold upd_pq_state. destruct (Z.eq_dec v u). subst v. exfalso; apply n. apply in_or_app; right; left; auto.
     rewrite upd_Znth_diff. rewrite Hinv_6 by lia. destruct (in_dec V_EqDec v popped_vertices). exfalso; apply n. apply in_or_app; left; auto.
-    rewrite Hinv_5 by lia. auto.
+    rewrite Hinv_5 by lia. destruct (V_EqDec v r). contradiction. auto.
     replace (Zlength pq_state) with SIZE by lia. lia.
     replace (Zlength pq_state) with SIZE by lia. lia. auto.
     ****
@@ -813,6 +847,14 @@ break: (
     replace (Zlength pq_state) with SIZE; lia. replace (Zlength pq_state) with SIZE; lia.
     unfold not; intros. subst v. apply n. apply in_or_app; right; left; auto.
   }
+  assert (Hpopped_nil: popped_vertices +:: u = [] -> r = (@find V V_EqDec) pq_state' (fold_right Z.min (hd 0 pq_state') pq_state') 0). {
+    intros. assert (In u (popped_vertices+::u)). apply in_or_app; right; left; auto.
+    rewrite H5 in H6. contradiction.
+  }
+  assert (Hpopped_unnil: popped_vertices +:: u <> [] -> hd_error (popped_vertices +:: u) = Some r). {
+    intros. destruct popped_vertices. rewrite Hur; auto.
+    apply hd_error_app. rewrite Hr2; auto. unfold not; intros. inversion H6.
+  }
   assert (Hheavy: forall v : Z, 0 <= v < SIZE -> 0 <= Znth v parents' < SIZE ->
     evalid g (eformat (v, Znth v parents')) /\
     (exists i : Z, 0 <= i < Zlength (popped_vertices +:: u) /\
@@ -839,7 +881,7 @@ break: (
     destruct (V_EqDec v u).
     (*subcase v = u*) hnf in e. subst v.
     replace ((@find V V_EqDec) (popped_vertices +:: u) u 0) with (Zlength popped_vertices) in H11.
-    replace (find popped_vertices u 0) with (Zlength popped_vertices). auto.
+    replace ((@find V V_EqDec) popped_vertices u 0) with (Zlength popped_vertices). auto.
     rewrite find_notIn_0; auto.
     rewrite find_app_notIn1. rewrite find_cons. rewrite Z.add_0_r. auto. auto.
     (*subcase v <> u*) unfold RelationClasses.complement, Equivalence.equiv in c.
@@ -873,7 +915,10 @@ break: (
       2: replace (Zlength pq_state) with SIZE; lia. 2: auto.
       rewrite Hinv_6 in bool. 2: lia. destruct (in_dec V_EqDec v popped_vertices).
       exfalso. apply n. apply in_or_app; left; auto.
-      rewrite Hinv_5 in bool by lia.
+      rewrite Hinv_5 in bool by lia. destruct (V_EqDec v r). hnf in e; subst v.
+      destruct popped_vertices. exfalso; apply H10; symmetry; apply Hur. auto.
+      assert (hd_error (v :: popped_vertices) = Some r). apply Hr2. unfold not; intros; inversion H11.
+      inversion H11. subst v. exfalso; apply n. apply in_or_app; left; left; auto.
       (*now check whether Znth v parents is SIZE or lower.
         If < SIZE, use Hinv_7 to show that eformat(u0,v) must be bigger than parents.
         If SIZE, use Hinv_8 to derive that eformat(u0,v) is invalid.
@@ -919,7 +964,11 @@ break: (
       2: replace (Zlength pq_state) with SIZE; lia. 2: replace (Zlength pq_state) with SIZE; lia.
       2: auto.
       rewrite Hinv_6 in bool by lia. destruct (in_dec V_EqDec v popped_vertices). exfalso; apply n; apply in_or_app; left; auto.
-      rewrite Hinv_5 in bool by lia.
+      rewrite Hinv_5 in bool by lia. destruct (V_EqDec v r).
+      (*v=r*)hnf in e; subst v. (*hm...*)
+      exfalso; apply n. apply hd_error_In. apply Hpopped_unnil. unfold not; intros.
+      assert (In u (popped_vertices+::u)). apply in_or_app; right; left; auto. rewrite H13 in H14; contradiction.
+      (*v<>r*)
       rewrite graph_to_mat_eq in bool by lia. apply bool.
     (*finally, non adjacent*)
     replace (Znth v parents') with (Znth v parents). 2: symmetry; apply Hinv2_1; auto.
@@ -985,10 +1034,13 @@ break: (
     rewrite Z.ltb_ge in bool. unfold upd_pq_state in bool.
     rewrite upd_Znth_diff in bool. rewrite Hinv_6 in bool by lia.
     destruct (in_dec V_EqDec v popped_vertices). exfalso; apply n; apply in_or_app; left; auto.
-    rewrite Hinv_5 in bool by lia.
-    replace (elabel g (eformat (v, Znth v parents))) with inf in bool. lia.
-    symmetry; apply invalid_edge_weight.
+    rewrite Hinv_5 in bool by lia. destruct (V_EqDec v r).
+    hnf in e; subst v. exfalso; apply n. apply hd_error_In. apply Hpopped_unnil.
+    unfold not; intros. assert (In u (popped_vertices+::u)). apply in_or_app; right; left; auto.
+    rewrite H8 in H9; contradiction.
+    assert (elabel g (eformat (v,Znth v parents)) = inf). apply invalid_edge_weight.
     unfold not; intros. apply eformat_evalid_vvalid in H8. destruct H8. rewrite H6 in H9. rewrite vert_bound in H9. lia.
+    rewrite H8 in bool. lia.
     replace (Zlength pq_state) with SIZE; lia.
     replace (Zlength pq_state) with SIZE; lia.
     unfold not; intros; subst v. apply n; apply in_or_app; right; left; auto.
@@ -1008,11 +1060,11 @@ break: (
     apply in_app_or in H5. destruct H5.
     (*case was already in popped vertices*)
     rewrite find_app_In1 in H8, H9 by auto. rewrite sublist_app1 in H8, H9.
-      2: pose proof ((@find_lbound V V_EqDec) popped_vertices v 0); lia.
+      2: { pose proof ((@find_lbound V V_EqDec) popped_vertices v 0); lia. }
       2: { pose proof ((@find_ubound V V_EqDec) popped_vertices v 0). rewrite Z.add_0_r in H11. auto. }
-      2: pose proof ((@find_lbound V V_EqDec) popped_vertices v 0); lia.
+      2: { pose proof ((@find_lbound V V_EqDec) popped_vertices v 0); lia. }
       2: { pose proof ((@find_ubound V V_EqDec) popped_vertices v 0). rewrite Z.add_0_r in H11. auto. }
-    apply Hinv_12; auto.
+    apply Hinv_14; auto.
     (*case v = u*)
     destruct H5. 2: contradiction. subst v.
     assert ((sublist 0 ((@find V V_EqDec) (popped_vertices +:: u) u 0) (popped_vertices +:: u)) =
@@ -1043,18 +1095,26 @@ break: (
     2: { assert (~ adjacent g u1 u2). apply Hinv_8. lia. lia.
           rewrite find_notIn, Z.add_0_r, sublist_same by auto. auto.
         rewrite eformat_adj in H14. apply invalid_edge_weight in H14.
-        rewrite H14. apply weight_inf_bound. }
+        replace (elabel g (eformat (u1, u2))) with inf. apply weight_inf_bound. }
     (*u2 <> u*) unfold RelationClasses.complement, Equivalence.equiv in c.
     assert (Znth u pq_state <= Znth u2 pq_state). apply Hu_min; lia.
     rewrite (Hinv_6 u2) in H14 by lia. destruct (in_dec V_EqDec u2 popped_vertices). contradiction.
-    clear n. rewrite Hinv_5 in H14.
+    clear n. rewrite Hinv_5 in H14. destruct (V_EqDec u2 r).
+    hnf in e. subst u2. destruct popped_vertices. contradiction. exfalso; apply H9.
+    apply hd_error_In. apply Hr2. unfold not; intros. assert (In v (v::popped_vertices)) by (left; auto).
+    rewrite H15 in H16; contradiction.
+    unfold RelationClasses.complement, Equivalence.equiv in c0.
     assert (elabel g (eformat (u2, Znth u2 parents)) <= elabel g (eformat (u1,u2))).
       apply Hinv_7. lia. lia. rewrite find_notIn, Z.add_0_r, sublist_same by auto. auto. 2: auto.
     apply (Z.le_trans _ (elabel g (eformat (u2, Znth u2 parents)))). 2: auto.
     apply (Z.le_trans _ (Znth u pq_state)). 2: auto.
     clear H14 H15.
     rewrite Hinv_6 by lia. destruct (in_dec V_EqDec u popped_vertices). contradiction.
-    rewrite Hinv_5 by lia. apply Z.le_refl.
+    rewrite Hinv_5 by lia. destruct (V_EqDec u r).
+    hnf in e; subst u. destruct popped_vertices. contradiction. exfalso; apply n.
+    apply hd_error_In. apply Hr2. unfold not; intros. assert (In v (v::popped_vertices)). left; auto.
+    rewrite H14 in H15; contradiction.
+    apply Z.le_refl.
   }
   (*now split into cases*)
   apply Z.le_lteq in H4. destruct H4.
@@ -1078,7 +1138,7 @@ break: (
     split. apply weight_representable. apply evalid_inf_iff; auto.
   }
   assert (Hu_evalid: ~ evalid mst' (eformat (u,(Znth u parents)))). {
-    unfold not; intros. apply (Hinv_11 u (Znth u parents)).
+    unfold not; intros. apply (Hinv_13 u (Znth u parents)).
     auto. rewrite eformat_adj. auto.
   }
   assert (Huparents_popped: In (Znth u parents) popped_vertices). {
@@ -1095,19 +1155,19 @@ break: (
   Exists (finGraph adde_u).
   Exists parents' keys' pq_state' (popped_vertices+::u) (remove V_EqDec u unpopped_vertices).
   assert (HM: exists M : MatrixUGraph, minimum_spanning_forest M g /\ is_partial_lgraph adde_u M). {
-    destruct Hinv_13 as [M [Hmsf_M Hpartial_M]]. pose proof (finGraph M).
+    destruct Hinv_15 as [M [Hmsf_M Hpartial_M]]. pose proof (finGraph M).
     destruct (evalid_dec M (eformat (u, Znth u parents))).
     ****
       exists M. split. auto. apply adde_partial_lgraph; auto. rewrite <- surjective_pairing; auto.
       rewrite <- surjective_pairing. symmetry. apply Hmsf_M; auto.
     ****
       set (a:=eformat (u, Znth u parents)) in *.
-      (*(@find V V_EqDec) a corresponding edge b in M, show that elabel g a <= elabel g b
+      (*find a corresponding edge b in M, show that elabel g a <= elabel g b
         Then do a swap
       *)
       assert (connected M (Znth u parents) u). apply Hmsf_M. apply adjacent_connected. exists a.
         split. apply evalid_strong_evalid; auto.
-        rewrite src_fst, dst_snd.
+        rewrite src_fst, dst_snd; auto.
         unfold a; destruct (Z.le_ge_cases u (Znth u parents)). rewrite eformat1 by (simpl; auto).
         simpl. right. auto.
         rewrite eformat2 by (simpl; auto). simpl. left; auto.
@@ -1161,9 +1221,9 @@ break: (
         unfold b in H17. apply eformat_eq in H17. destruct H17; destruct H17; subst v1; subst v2; contradiction.
         apply Hinv_9.
       }
-      clear Hinv_1 Hinv_2 Hinv_3 Hinv_4 Hinv_5 Hinv_6 Hinv_7 Hinv_8 Hinv_9 Hinv_10 Hinv_11 Hinv_12.
-      clear Hinv2_1 Hinv2_2 Hinv2_3 Hparents_bound Hkeys' Hpq_state' Hheavy Hheavy2 Hweight.
-      clear Hpopped_or_unpopped Hpopped_vvalid Hunpopped_vvalid Hu_not_popped Hu_unpopped Hu_min HZlength_parents HZlength_keys HZlength_pq_state Hu_parents Hu_keys Hu_pq_state Huparents_popped Huparents_unpopped.
+      clear Hinv_1 Hinv_2 Hinv_3 Hinv_4 Hinv_5 Hinv_6 Hinv_7 Hinv_8 Hinv_9 Hinv_10 Hr1 Hr2 Hinv_13 Hinv_14.
+      clear Hinv2_1 Hinv2_2 Hinv2_3 Hparents_bound Hkeys' Hpq_state' Hheavy Hheavy2 Hweight Hpopped_nil Hpopped_unnil.
+      clear Hpopped_or_unpopped Hpopped_vvalid Hunpopped_vvalid Hu_not_popped Hu_unpopped Hur Hu_min HZlength_parents HZlength_keys HZlength_pq_state Hu_parents Hu_keys Hu_pq_state Huparents_popped Huparents_unpopped.
       set (remove_b:= eremove M b). (*huh, how come I don't need to provide evalid b?*)
       assert (Ha_fst_vvalid: vvalid remove_b (fst a)). {
         unfold a; simpl. destruct (Z.le_ge_cases u (Znth u parents)).
@@ -1303,7 +1363,7 @@ break: (
           ++ (*b is in l', must take detour*)
           assert (In b l'); auto. apply (fits_upath_split2 M p' l' b x y) in H; auto.
           destruct H as [p1x [p2y [l1x [l2y [? [? [? [? ?]]]]]]]]. subst l'; subst p'.
-          rewrite src_fst, dst_snd in H0 by auto.
+          rewrite src_fst, dst_snd in H0.
           assert (~ In b l1x). { unfold not; intros. apply (NoDup_app_not_in _ l1x ([b]++l2y) H27 b) in H. apply H. apply in_or_app; left; left; auto. }
           assert (~ In b l2y). { apply NoDup_app_r in H27. apply (NoDup_app_not_in _ [b] l2y H27 b). left; auto. }
           destruct H0; destruct H0.
@@ -1371,7 +1431,7 @@ break: (
       destruct p. inversion H11; inversion H12. subst v.
       rewrite H15 in Hu_unpopped; contradiction.
       destruct H9. inversion H11. subst v.
-      apply (Hinv_11 u v0). auto. apply H9.
+      apply (Hinv_13 u v0). auto. apply H9.
       ****
       rewrite eformat2 in *; try (simpl; lia).
       simpl in H9. apply connected_symm in H9.
@@ -1379,7 +1439,7 @@ break: (
       destruct p. inversion H11; inversion H12. subst v.
       rewrite H15 in Hu_unpopped; contradiction.
       destruct H9. inversion H11. subst v.
-      apply (Hinv_11 u v0). auto. apply H9.
+      apply (Hinv_13 u v0). auto. apply H9.
   }
   assert (Hu_new: evalid adde_u (eformat (u, Znth u parents))). {
     simpl. unfold graph_gen.addValidFunc. right; rewrite <- surjective_pairing. auto. }
@@ -1389,7 +1449,7 @@ break: (
     apply dst_snd. }
   assert (Hnot_adj: forall u0 v : V, In u0 (remove V_EqDec u unpopped_vertices) -> ~ adjacent adde_u u0 v). {
     intros. rewrite remove_In_iff in H9; destruct H9.
-    assert (~ adjacent mst' u0 v). apply Hinv_11. auto.
+    assert (~ adjacent mst' u0 v). apply Hinv_13. auto.
     unfold not; intros. destruct H12 as [e ?]. destruct (E_EqDec (eformat (u,Znth u parents)) e).
     hnf in e0. subst e.
     destruct H12. rewrite Hsrc, Hdst in H13.
@@ -1439,7 +1499,7 @@ break: (
   }
   time "end of pop loop (adde_u) (did not record original):" entailer!.
   clear H9 H10 H11 H12 H13 H14 H15 H16 H17 H18 H19 H20 H21 H22 Pv_pq HPv_pq Pv_pq0 Pv_out HPv_out Pv_out0 Pv_key HPv_key Pv_key0.
-
+  split.
   (*permutation of EList*)
     apply (Permutation_trans (l':=(eformat (u,Znth u parents))::(EList mst'))).
     apply Permutation_sym.
@@ -1478,6 +1538,7 @@ break: (
     apply Hpopped_vvalid; auto.
     destruct H9. 2: contradiction. subst a. apply Hunpopped_vvalid; auto.
     right; auto.
+    intros. assert (In u (popped_vertices +:: u)). apply in_or_app; right; left; auto. rewrite H9 in H10; contradiction.
   ++ (*Znth u keys = inf. Implies u has no other vertices from the mst that can connect to it. Thus, no change to graph*)
   Exists mst' fmst' parents' keys' pq_state' (popped_vertices+::u) (remove V_EqDec u unpopped_vertices).
   assert (Permutation (EList mst')
@@ -1539,11 +1600,19 @@ break: (
         assert (Znth u pq_state = Znth u keys). rewrite Hinv_6 by lia.
           destruct (in_dec V_EqDec u popped_vertices). contradiction. auto.
         assert (Znth u keys <= Znth v2 keys). rewrite <- H15, <- H16. apply Hu_min; lia.
-        assert (Znth v2 keys < inf). rewrite Hinv_5 by lia.
+        assert (Znth v2 keys < inf). rewrite Hinv_5 by lia. destruct (V_EqDec v2 r). rewrite inf_eq; lia.
           apply strong_inf_bound. apply Hinv_7; lia.
         (*now so Znth u keys = inf*)
         destruct popped_vertices. contradiction.
-        assert( Znth u keys = elabel g (eformat (u,Znth u parents))). rewrite Hinv_5 by lia. auto.
+        (*case u=r, then Znth v2 pq_state = Znth v2 keys should be = inf, lia. Easiest way to solve this is to hack Hinv_11*)
+        (*edit: ok that was unnecessary, lots of things to kill off u=r*)
+        (*case u<>r, then Znth u keys = elabel g (eformat (u, Znth u parents)), but Znth u parents = inf, so Znth u keys = inf. Then inf < inf*)
+        assert( Znth u keys = elabel g (eformat (u,Znth u parents))). rewrite Hinv_5 by lia.
+        destruct (V_EqDec u r). hnf in e.
+          assert (In r (v::popped_vertices)). apply hd_error_In. apply Hr2.
+          unfold not; intros. assert (In v (v::popped_vertices)). left; auto.
+          rewrite H19 in H20; contradiction. subst u. contradiction.
+          auto.
         rewrite H19 in H17. replace (elabel g (eformat (u, Znth u parents))) with inf in H17. lia.
         symmetry; apply invalid_edge_weight.
         unfold not; intros. rewrite H4 in H20. apply eformat_evalid_vvalid in H20. destruct H20.
@@ -1554,7 +1623,7 @@ break: (
       auto. auto.
       (*mst' -> g*) apply connected_symm in H7. destruct H7 as [p [? [? ?]]]. destruct p. inversion H8.
       inversion H8. destruct p. inversion H9. subst v. subst u0. apply connected_refl. rewrite vert_bound; lia.
-      subst v. destruct H7. exfalso. apply (Hinv_11 u v0); auto.
+      subst v. destruct H7. exfalso. apply (Hinv_13 u v0); auto.
     ****(*u0=u, which is repeat of above*) destruct H6. 2: contradiction. subst u0. rename H7 into H6.
       split; intros.
       (*g -> mst'*)
@@ -1581,11 +1650,19 @@ break: (
         assert (Znth u pq_state = Znth u keys). rewrite Hinv_6 by lia.
           destruct (in_dec V_EqDec u popped_vertices). contradiction. auto.
         assert (Znth u keys <= Znth v2 keys). rewrite <- H15, <- H16. apply Hu_min; lia.
-        assert (Znth v2 keys < inf). rewrite Hinv_5 by lia.
+        assert (Znth v2 keys < inf). rewrite Hinv_5 by lia. destruct (V_EqDec v2 r). rewrite inf_eq; lia.
           apply strong_inf_bound. apply Hinv_7; lia.
         (*now so Znth u keys = inf*)
         destruct popped_vertices. contradiction.
-        assert( Znth u keys = elabel g (eformat (u,Znth u parents))). rewrite Hinv_5 by lia. auto.
+        (*case u=r, then Znth v2 pq_state = Znth v2 keys should be = inf, lia. Easiest way to solve this is to hack Hinv_11*)
+        (*edit: ok that was unnecessary, lots of things to kill off u=r*)
+        (*case u<>r, then Znth u keys = elabel g (eformat (u, Znth u parents)), but Znth u parents = inf, so Znth u keys = inf. Then inf < inf*)
+        assert( Znth u keys = elabel g (eformat (u,Znth u parents))). rewrite Hinv_5 by lia.
+        destruct (V_EqDec u r). hnf in e.
+          assert (In r (v0::popped_vertices)). apply hd_error_In. apply Hr2.
+          unfold not; intros. assert (In v0 (v0::popped_vertices)). left; auto.
+          rewrite H19 in H20; contradiction. subst u. contradiction.
+          auto.
         rewrite H19 in H17. replace (elabel g (eformat (u, Znth u parents))) with inf in H17. lia.
         symmetry; apply invalid_edge_weight.
         unfold not; intros. rewrite H4 in H20. apply eformat_evalid_vvalid in H20. destruct H20.
@@ -1596,21 +1673,23 @@ break: (
       auto. auto.
       (*mst' -> g*) destruct H7 as [p [? [? ?]]]. destruct p. inversion H8.
       inversion H8. destruct p. inversion H9. subst v0. subst v. apply connected_refl. rewrite vert_bound; lia.
-      subst v0. destruct H7. exfalso. apply (Hinv_11 u v1); auto.
+      subst v0. destruct H7. exfalso. apply (Hinv_13 u v1); auto.
     ****(*both=u*)destruct H6. 2: contradiction. destruct H7. 2: contradiction. subst u0; subst v.
     split; intros; apply connected_refl; rewrite vert_bound; lia.
   }
   assert (Hnot_adj: forall u0 v : V, In u0 (remove V_EqDec u unpopped_vertices) -> ~ adjacent mst' u0 v). {
-    intros. apply Hinv_11. rewrite remove_In_iff in H6; apply H6.
+    intros. apply Hinv_13. rewrite remove_In_iff in H6; apply H6.
   }
   time "End of pop loop (same msf) (originally 150s):" entailer!.
+  assert (In u (popped_vertices+::u)). apply in_or_app; right; left; auto. rewrite H20 in H21; contradiction.
   }
   { (*break*) forward. (*no more vertices in queue*)
     assert (Hempty: (@isEmpty inf) pq_state = Vone). {
       destruct ((@isEmptyTwoCases inf) pq_state);
       rewrite H1 in H0; simpl in H0; now inversion H0.
     } clear H0.
-    apply (@isEmptyMeansInf inf) in Hempty. rename Hempty into H0. rewrite Forall_forall in H0.
+    rewrite ((@isEmptyMeansInf inf)) in Hempty.
+    rewrite Forall_forall in Hempty. rename Hempty into H0.
     assert (Permutation popped_vertices (VList mst')). {
       apply NoDup_Permutation.
       apply Permutation_sym, Permutation_NoDup, NoDup_app_l in Hinv_3. auto. apply NoDup_VList.
@@ -1620,6 +1699,7 @@ break: (
       assert (Znth x pq_state = (if in_dec V_EqDec x popped_vertices then inf + 1 else Znth x keys)). apply Hinv_6; auto.
       destruct (in_dec V_EqDec x popped_vertices). auto. exfalso. rewrite Hinv_5 in H2.
       assert (Znth x pq_state > inf). apply H0. apply Znth_In. rewrite HZlength_pq_state. auto. 2: auto.
+      destruct (V_EqDec x r). rewrite inf_eq in H3; lia.
       rewrite H2 in H3. pose proof (weight_inf_bound g (eformat (x, Znth x parents))).
       (*how now brown cow, I can't lia*)
       apply Zgt_not_le in H3. contradiction.
@@ -1659,6 +1739,13 @@ break: (
       apply (Permutation_in (l:=VList mst')). apply Permutation_sym; auto. apply H3.
       apply (Permutation_in (l:=VList mst')). apply Permutation_sym; auto. apply H4.
     }
+    assert (hd_error popped_vertices = Some r). {
+      destruct popped_vertices. assert (vvalid mst' 0). rewrite vert_bound; lia.
+      rewrite <- VList_vvalid in H3. apply (Permutation_in (l':=[])) in H3. contradiction.
+      apply Permutation_sym; apply H1.
+      apply Hr2. unfold not; intros. assert (In v (v::popped_vertices)) by (left; auto).
+      rewrite H3 in H4; contradiction.
+    }
     time entailer!. (*was 55 seconds without PROP*)
   }
 }
@@ -1669,7 +1756,8 @@ rename H into Hinv_1; rename H0 into Hinv_2;
 rename H1 into Hinv_3; rename H2 into Hinv_4;
 rename H3 into Hinv_5; rename H4 into Hinv_6;
 rename H5 into Hinv_7; rename H6 into Hinv_8;
-rename H7 into Hinv_9; rename H8 into Hinv_10.
+rename H7 into Hinv_9; rename H8 into Hinv_10;
+rename H9 into Hinv_11.
 (*Do the minimum proof here*)
 assert (labeled_spanning_uforest mst g). {
   split. split. apply Hinv_1. split. apply Hinv_2. apply Hinv_7.
@@ -1677,7 +1765,7 @@ assert (labeled_spanning_uforest mst g). {
   unfold preserve_elabel; intros. apply Hinv_1. auto.
 }
 assert (minimum_spanning_forest mst g). {
-  destruct Hinv_10 as [M [? ?]].
+  destruct Hinv_11 as [M [? ?]].
   apply (partial_lgraph_spanning_mst mst M g); auto.
 }
 assert (Permutation (EList mst)
@@ -1698,6 +1786,5 @@ Exists mst fmst parents.
 (*change from popped_vertices to nat_inc_list*)
 entailer!.
 }
-(*huh, where did I forget this*) rewrite map_list_repeat; auto.
 (*Should we bother with filling a matrix for it? The original Prim doesn't bother*)
 Qed.
